Working on ConsistentRefs

AllRefs.v
@@ -6,7 +6,7 @@ From Elo Require Import Util.
 From Elo Require Import Array.
 From Elo Require Import Map.
 From Elo Require Import Core.
-From Elo Require Import ValidAccesses.
+From Elo Require Import ValidAddresses.
 From Elo Require Import References.
 
 Inductive RefType : Prop :=
@@ -15,326 +15,212 @@ Inductive RefType : Prop :=
   .
 
 (* -------------------------------------------------------------------------- *)
-(* has-address                                                                *)
-(* -------------------------------------------------------------------------- *)
-
-Inductive HasAddress (ad : addr) : tm -> Prop :=
-  | hasad_ref : forall T,
-    HasAddress ad <{ &ad :: T }>
-
-  | hasad_new : forall t T,
-    HasAddress ad t ->
-    HasAddress ad <{ new T t }>
-
-  | hasad_load : forall t,
-    HasAddress ad t ->
-    HasAddress ad <{ *t }>
-
-  | hasad_asg1 : forall t1 t2,
-    HasAddress ad t1 ->
-    HasAddress ad <{ t1 = t2 }>
-
-  | hasad_asg2 : forall t1 t2,
-    HasAddress ad t2 ->
-    HasAddress ad <{ t1 = t2 }>
-
-  | hasad_fun : forall t x Tx,
-    HasAddress ad t ->
-    HasAddress ad <{ fn x Tx --> t }>
-
-  | hasad_call1 : forall t1 t2,
-    HasAddress ad t1 ->
-    HasAddress ad <{ call t1 t2 }>
-
-  | hasad_call2 : forall t1 t2,
-    HasAddress ad t2 ->
-    HasAddress ad <{ call t1 t2 }>
-
-  | hasad_seq1 : forall t1 t2,
-    HasAddress ad t1 ->
-    HasAddress ad <{ t1; t2 }>
-
-  | hasad_seq2 : forall t1 t2,
-    HasAddress ad t2 ->
-    HasAddress ad <{ t1; t2 }>
-
-  | hasad_spawn : forall t,
-    HasAddress ad t ->
-    HasAddress ad <{ spawn t }>
-  .
-
-Local Lemma hasad_dec : forall ad t,
-  Decidable.decidable (HasAddress ad t).
-Proof. intros. eauto using classic_decidable. Qed.
-
-Local Ltac solve_inv_nha1 :=
-  intros; intros ?; eauto using HasAddress.
-
-Local Ltac solve_inv_nha2 :=
-  intros * F; eapply Classical_Prop.not_or_and;
-  intros [? | ?]; eapply F; eauto using HasAddress.
-
-Local Lemma inv_nha_ref : forall ad ad' T,
-  ~ HasAddress ad <{ &ad' :: T}> ->
-  ad <> ad'.
-Proof. intros. intros ?. subst. eauto using HasAddress. Qed.
-
-Local Lemma inv_nha_new : forall ad t T,
-  ~ HasAddress ad <{ new T t }> ->
-  ~ HasAddress ad t.
-Proof. solve_inv_nha1. Qed.
-
-Local Lemma inv_nha_load : forall ad t,
-  ~ HasAddress ad <{ *t }> ->
-  ~ HasAddress ad t.
-Proof. solve_inv_nha1. Qed.
-
-Local Lemma inv_nha_asg : forall ad t1 t2,
-  ~ HasAddress ad <{ t1 = t2 }> ->
-  (~ HasAddress ad t1) /\ (~ HasAddress ad t2).
-Proof. solve_inv_nha2. Qed.
-
-Local Lemma inv_nha_fun : forall ad t x Tx,
-  ~ HasAddress ad <{ fn x Tx --> t }> ->
-  ~ HasAddress ad t.
-Proof. solve_inv_nha1. Qed.
-
-Local Lemma inv_nha_call : forall ad t1 t2,
-  ~ HasAddress ad <{ call t1 t2 }> ->
-  (~ HasAddress ad t1) /\ (~ HasAddress ad t2).
-Proof. solve_inv_nha2. Qed.
-
-Local Lemma inv_nha_seq : forall ad t1 t2,
-  ~ HasAddress ad <{ t1; t2 }> ->
-  (~ HasAddress ad t1) /\ (~ HasAddress ad t2).
-Proof. solve_inv_nha2. Qed.
-
-Local Lemma inv_nha_spawn : forall ad t,
-  ~ HasAddress ad <{ spawn t }> ->
-  ~ HasAddress ad t.
-Proof. solve_inv_nha1. Qed.
-
-Local Ltac inversion_nha :=
-  match goal with
-  | H : ~ HasAddress _ <{ & _ :: _ }> |- _ => eapply inv_nha_ref in H
-  | H : ~ HasAddress _ <{ new _ _  }> |- _ => eapply inv_nha_new  in H
-  | H : ~ HasAddress _ <{ * _      }> |- _ => eapply inv_nha_load in H
-  | H : ~ HasAddress _ <{ _ = _    }> |- _ => eapply inv_nha_asg  in H as [? ?]
-  | H : ~ HasAddress _ <{ fn _ _ --> _ }> |- _ => eapply inv_nha_fun in H
-  | H : ~ HasAddress _ <{ call _ _ }> |- _ => eapply inv_nha_call  in H as [? ?]
-  | H : ~ HasAddress _ <{ _ ; _    }> |- _ => eapply inv_nha_seq   in H as [? ?]
-  | H : ~ HasAddress _ <{ spawn _  }> |- _ => eapply inv_nha_spawn in H
-  end.
-
-(* -------------------------------------------------------------------------- *)
-(* terms                                                                      *)
+(* consistent-refs                                                            *)
 (* -------------------------------------------------------------------------- *)
 
 (*
-  | forall_refs_refI : forall T,
-    ForallRefs ad T <{ &ad :: T }>
+  | conrefs_ref : forall T,
+    ConsistentRefs ad T <{ &ad :: T }>
 *)
 
-Inductive ForallRefs (ad : addr) : RefType -> tm -> Prop :=
-  | forall_refs_unit : forall rt,
-    ForallRefs ad rt <{ unit }>
+Inductive ConsistentRefs (ad : addr) : RefType -> tm -> Prop :=
+  | conrefs_unit : forall rt,
+    ConsistentRefs ad rt <{ unit }>
 
-  | forall_refs_num : forall rt n,
-    ForallRefs ad rt <{ N n }>
+  | conrefs_num : forall rt n,
+    ConsistentRefs ad rt <{ N n }>
 
-  | forall_refs_ref : forall rt ad' T,
+  | conrefs_ref : forall rt ad' T,
     ad <> ad' ->
-    ForallRefs ad rt <{ &ad' :: T }>
+    ConsistentRefs ad rt <{ &ad' :: T }>
 
-  | forall_refs_refI : forall T,
-    ForallRefs ad Immut <{ &ad :: i&T }>
+  | conrefs_refI : forall T,
+    ConsistentRefs ad Immut <{ &ad :: i&T }>
 
-  | forall_refs_refM : forall T,
-    ForallRefs ad Mut <{ &ad :: &T }>
+  | conrefs_refM : forall T,
+    ConsistentRefs ad Mut <{ &ad :: &T }>
 
-  | forall_refs_new : forall rt t T,
-    ForallRefs ad rt t ->
-    ForallRefs ad rt <{ new T t }>
+  | conrefs_new : forall rt t T,
+    ConsistentRefs ad rt t ->
+    ConsistentRefs ad rt <{ new T t }>
 
-  | forall_refs_load : forall rt t,
-    ForallRefs ad rt t ->
-    ForallRefs ad rt <{ *t }>
+  | conrefs_load : forall rt t,
+    ConsistentRefs ad rt t ->
+    ConsistentRefs ad rt <{ *t }>
 
-  | forall_refs_asg : forall rt t1 t2,
-    ForallRefs ad rt t1 ->
-    ForallRefs ad rt t2 ->
-    ForallRefs ad rt <{ t1 = t2 }>
+  | conrefs_asg : forall rt t1 t2,
+    ConsistentRefs ad rt t1 ->
+    ConsistentRefs ad rt t2 ->
+    ConsistentRefs ad rt <{ t1 = t2 }>
 
-  | forall_refs_var : forall rt x,
-    ForallRefs ad rt <{ var x }>
+  | conrefs_var : forall rt x,
+    ConsistentRefs ad rt <{ var x }>
 
-  | forall_refs_fun : forall rt t x Tx,
-    ForallRefs ad rt t ->
-    ForallRefs ad rt <{ fn x Tx --> t }>
+  | conrefs_fun : forall rt t x Tx,
+    ConsistentRefs ad rt t ->
+    ConsistentRefs ad rt <{ fn x Tx --> t }>
 
-  | forall_refs_call : forall rt t1 t2,
-    ForallRefs ad rt t1 ->
-    ForallRefs ad rt t2 ->
-    ForallRefs ad rt <{ call t1 t2 }>
+  | conrefs_call : forall rt t1 t2,
+    ConsistentRefs ad rt t1 ->
+    ConsistentRefs ad rt t2 ->
+    ConsistentRefs ad rt <{ call t1 t2 }>
 
-  | forall_refs_seq : forall rt t1 t2,
-    ForallRefs ad rt t1 ->
-    ForallRefs ad rt t2 ->
-    ForallRefs ad rt <{ t1; t2 }>
+  | conrefs_seq : forall rt t1 t2,
+    ConsistentRefs ad rt t1 ->
+    ConsistentRefs ad rt t2 ->
+    ConsistentRefs ad rt <{ t1; t2 }>
 
-  | forall_refs_spawn : forall rt t,
-    ForallRefs ad rt t ->
-    ForallRefs ad rt <{ spawn t }>
+  | conrefs_spawn : forall rt t,
+    ConsistentRefs ad rt t ->
+    ConsistentRefs ad rt <{ spawn t }>
   .
 
-Definition ForallRefsMem (m : mem) (rt : RefType) := forall ad,
-  forall_memory m (ForallRefs ad rt).
+Definition ConsistentRefsMem (m : mem) (rt : RefType) := forall ad,
+  forall_memory m (ConsistentRefs ad rt).
 
 (* -------------------------------------------------------------------------- *)
 (* properties                                                                 *)
 (* -------------------------------------------------------------------------- *)
 
-Local Lemma not_hasad_then_forall_refs : forall rt t ad,
+Local Lemma nha_then_conrefs : forall rt t ad,
   ~ HasAddress ad t ->
-  ForallRefs ad rt t.
+  ConsistentRefs ad rt t.
 Proof.
-  intros. induction t; try inversion_nha; eauto using ForallRefs.
+  intros. induction t; try inversion_nha; eauto using ConsistentRefs.
 Qed.
 
 (* -------------------------------------------------------------------------- *)
 (* valid-references                                                           *)
 (* -------------------------------------------------------------------------- *)
 
-Definition valid_references (rt : RefType) (t : tm) := forall ad,
-  HasAddress ad t -> ForallRefs ad rt t.
-
-(* -------------------------------------------------------------------------- *)
-(* constructor-vr                                                             *)
-(* -------------------------------------------------------------------------- *)
+Definition valid_references (rt : RefType) (ad : addr) (t : tm) :=
+  HasAddress ad t -> ConsistentRefs ad rt t.
 
 Local Ltac solve_con_vr1 :=
-  intros * ? ? Hha; inversion_subst_clear Hha; eauto using ForallRefs.
+  intros; intros ?; inversion_ha; eauto using ConsistentRefs.
 
 Local Ltac solve_con_vr2 :=
-  intros * ? ? ? Hha; inversion_subst_clear Hha; eauto using ForallRefs;
+  intros; intros ?; inversion_ha; eauto using ConsistentRefs;
   match goal with
-  | _ : HasAddress ?ad ?tA |- ForallRefs _ _ (_ ?tA ?tB) =>
+  | _ : HasAddress ?ad ?tA |- ConsistentRefs _ _ (_ ?tA ?tB) =>
     destruct (hasad_dec ad tB)
-  | _ : HasAddress ?ad ?tA |- ForallRefs _ _ (_ ?tB ?tA) =>
+  | _ : HasAddress ?ad ?tA |- ConsistentRefs _ _ (_ ?tB ?tA) =>
     destruct (hasad_dec ad tB)
   end;
-  eauto using not_hasad_then_forall_refs, ForallRefs.
+  eauto using nha_then_conrefs, ConsistentRefs.
 
-Local Lemma vr_con_new : forall rt t T,
-  valid_references rt t ->
-  valid_references rt <{ new T t }>.
+Local Lemma vr_new : forall rt t ad T,
+  valid_references rt ad t ->
+  valid_references rt ad <{ new T t }>.
 Proof. solve_con_vr1. Qed.
 
-Local Lemma vr_con_load : forall rt t,
-  valid_references rt t ->
-  valid_references rt <{ *t }>.
+Local Lemma vr_load : forall rt t ad,
+  valid_references rt ad t ->
+  valid_references rt ad <{ *t }>.
 Proof. solve_con_vr1. Qed.
 
-Local Lemma vr_con_asg : forall rt t1 t2,
-  valid_references rt t1 ->
-  valid_references rt t2 ->
-  valid_references rt <{ t1 = t2 }>.
+Local Lemma vr_asg : forall rt t1 t2 ad,
+  valid_references rt ad t1 ->
+  valid_references rt ad t2 ->
+  valid_references rt ad <{ t1 = t2 }>.
 Proof. solve_con_vr2. Qed. 
 
-Local Lemma vr_con_call : forall rt t1 t2,
-  valid_references rt t1 ->
-  valid_references rt t2 ->
-  valid_references rt <{ call t1 t2 }>.
+Local Lemma vr_call : forall rt t1 t2 ad,
+  valid_references rt ad t1 ->
+  valid_references rt ad t2 ->
+  valid_references rt ad <{ call t1 t2 }>.
 Proof. solve_con_vr2. Qed. 
 
-Local Lemma vr_con_fun : forall rt t x Tx,
-  valid_references rt t ->
-  valid_references rt <{ fn x Tx --> t }>.
+Local Lemma vr_fun : forall rt t ad x Tx,
+  valid_references rt ad t ->
+  valid_references rt ad <{ fn x Tx --> t }>.
 Proof. solve_con_vr1. Qed. 
 
-Local Lemma vr_con_seq : forall rt t1 t2,
-  valid_references rt t1 ->
-  valid_references rt t2 ->
-  valid_references rt <{ t1; t2 }>.
+Local Lemma vr_seq : forall rt t1 t2 ad,
+  valid_references rt ad t1 ->
+  valid_references rt ad t2 ->
+  valid_references rt ad <{ t1; t2 }>.
 Proof. solve_con_vr2. Qed.
 
-Local Lemma vr_con_spawn : forall rt t,
-  valid_references rt t ->
-  valid_references rt <{ spawn t }>.
+Local Lemma vr_spawn : forall rt t ad,
+  valid_references rt ad t ->
+  valid_references rt ad <{ spawn t }>.
 Proof. solve_con_vr1. Qed.
 
 (* -------------------------------------------------------------------------- *)
-(* inversion-vad                                                              *)
+(* inversion-vr                                                               *)
 (* -------------------------------------------------------------------------- *)
 
 Local Ltac solve_inv_vr :=
-  intros * Hvr; try split; intros ad ?; specialize (Hvr ad);
+  intros * Hvr; try split; intros ?; unfold valid_references in *;
   unshelve (match goal with
-  | Hvr : HasAddress ad ?t -> _ |- _ =>
+  | Hvr : HasAddress ?ad ?t -> _ |- _ =>
     assert (Hhasad : HasAddress ad t) by shelve; specialize (Hvr Hhasad)
   end;
   inversion_subst_clear Hvr; assumption);
   eauto using HasAddress.
 
-Local Lemma inv_vr_new : forall rt t T,
-  valid_references rt <{ new T t }> ->
-  valid_references rt t.
+Local Lemma inv_vr_new : forall rt t ad T,
+  valid_references rt ad <{ new T t }> ->
+  valid_references rt ad t.
 Proof. solve_inv_vr. Qed.
 
-Local Lemma inv_vr_load : forall rt t,
-  valid_references rt <{ *t }> ->
-  valid_references rt t.
+Local Lemma inv_vr_load : forall rt t ad,
+  valid_references rt ad <{ *t }> ->
+  valid_references rt ad t.
 Proof. solve_inv_vr. Qed.
 
-Local Lemma inv_vr_asg : forall rt t1 t2,
-  valid_references rt <{ t1 = t2 }> ->
-  valid_references rt t1 /\ valid_references rt t2.
+Local Lemma inv_vr_asg : forall rt t1 t2 ad,
+  valid_references rt ad <{ t1 = t2 }> ->
+  valid_references rt ad t1 /\ valid_references rt ad t2.
 Proof. solve_inv_vr. Qed.
 
-Local Lemma inv_vr_call : forall rt t1 t2,
-  valid_references rt <{ call t1 t2 }> ->
-  valid_references rt t1 /\ valid_references rt t2.
+Local Lemma inv_vr_call : forall rt t1 t2 ad,
+  valid_references rt ad <{ call t1 t2 }> ->
+  valid_references rt ad t1 /\ valid_references rt ad t2.
 Proof. solve_inv_vr. Qed.
 
-Local Lemma inv_vr_fun : forall rt t x Tx,
-  valid_references rt <{ fn x Tx --> t }> ->
-  valid_references rt t.
+Local Lemma inv_vr_fun : forall rt t ad x Tx,
+  valid_references rt ad <{ fn x Tx --> t }> ->
+  valid_references rt ad t.
 Proof. solve_inv_vr. Qed.
 
-Local Lemma inv_vr_seq : forall rt t1 t2,
-  valid_references rt <{ t1; t2 }> ->
-  valid_references rt t1 /\ valid_references rt t2.
+Local Lemma inv_vr_seq : forall rt t1 t2 ad,
+  valid_references rt ad <{ t1; t2 }> ->
+  valid_references rt ad t1 /\ valid_references rt ad t2.
 Proof. solve_inv_vr. Qed.
 
-Local Lemma inv_vr_spawn : forall rt t,
-  valid_references rt <{ spawn t }> ->
-  valid_references rt t.
+Local Lemma inv_vr_spawn : forall rt t ad,
+  valid_references rt ad <{ spawn t }> ->
+  valid_references rt ad t.
 Proof. solve_inv_vr. Qed.
 
 Ltac inversion_vr :=
   match goal with
-  |H: valid_references _ <{ new _ _  }> |- _ => eapply inv_vr_new  in H
-  |H: valid_references _ <{ * _      }> |- _ => eapply inv_vr_load in H
-  |H: valid_references _ <{ _ = _    }> |- _ => eapply inv_vr_asg  in H as [? ?]
-  |H: valid_references _ <{ call _ _ }> |- _ => eapply inv_vr_call in H as [? ?]
-  |H: valid_references _ <{ fn _ _ --> _ }> |- _ => eapply inv_vr_fun in H
-  |H: valid_references _ <{ _; _     }> |- _ => eapply inv_vr_seq  in H as [? ?]
-  |H: valid_references _ <{ spawn _  }> |- _ => eapply inv_vr_spawn in H
+  | H : valid_references _ _ <{ new _ _      }> |- _ => eapply inv_vr_new  in H
+  | H : valid_references _ _ <{ * _          }> |- _ => eapply inv_vr_load in H
+  | H : valid_references _ _ <{ _ = _        }> |- _ =>
+                                                eapply inv_vr_asg  in H as [? ?]
+  | H : valid_references _ _ <{ call _ _     }> |- _ =>
+                                                eapply inv_vr_call in H as [? ?]
+  | H : valid_references _ _ <{ fn _ _ --> _ }> |- _ => eapply inv_vr_fun in H
+  | H : valid_references _ _ <{ _; _         }> |- _ =>
+                                                eapply inv_vr_seq  in H as [? ?]
+  | H : valid_references _ _ <{ spawn _      }> |- _ => eapply inv_vr_spawn in H
   end.
 
 (* -------------------------------------------------------------------------- *)
 (* subst                                                                      *)
 (* -------------------------------------------------------------------------- *)
 
-Local Lemma subst_vr : forall rt t tx x,
-  valid_references rt t ->
-  valid_references rt tx ->
-  valid_references rt ([x := tx] t).
+Local Lemma subst_vr : forall rt t tx ad x,
+  valid_references rt ad t ->
+  valid_references rt ad tx ->
+  valid_references rt ad ([x := tx] t).
 Proof.
   intros. induction t; eauto; try inversion_vr; simpl;
-  eauto using vr_con_new, vr_con_load, vr_con_asg, vr_con_call,
-    vr_con_seq, vr_con_spawn;
-  destruct String.string_dec; eauto using vr_con_fun.
+  eauto using vr_new, vr_load, vr_asg, vr_call, vr_seq, vr_spawn;
+  destruct String.string_dec; eauto using vr_fun.
 Qed.
 
 (* -------------------------------------------------------------------------- *)
@@ -357,41 +243,49 @@ Qed.
 *)
 
 (* -------------------------------------------------------------------------- *)
-(* vad-preservation                                                           *)
+(* vr-preservation                                                            *)
 (* -------------------------------------------------------------------------- *)
 
-Local Lemma step_none_vr_preservation : forall rt t t',
-  valid_references rt t ->
+Local Lemma step_none_vr_preservation : forall rt t t' ad,
+  valid_references rt ad t ->
   t --[EF_None]--> t' ->
-  valid_references rt t'.
+  valid_references rt ad t'.
 Proof.
   intros. induction_step; inversion_vr;
-  eauto using vr_con_new, vr_con_load, vr_con_asg, vr_con_call, vr_con_seq.
+  eauto using vr_new, vr_load, vr_asg, vr_call, vr_seq.
   inversion_vr. eauto using subst_vr. 
 Qed.
 
-Definition todo (rt : RefType) (t : tm) (ad : addr) :=
-  HasAddress ad t -> ForallRefs ad rt t.
-
-Local Lemma step_alloc_vr_preservation : forall rt m t t' ad v,
-  valid_accesses m t ->
-  HasAddress ad t ->
-  ForallRefs ad rt t ->
-  t --[EF_Alloc (@length tm m) v]--> t' ->
-  ForallRefs ad rt t'.
+Local Lemma step_alloc_vr_preservation1 : forall rt t t' ad ad' v,
+  ad <> ad' ->
+  ConsistentRefs ad rt t ->
+  t --[EF_Alloc ad' v]--> t' ->
+  ConsistentRefs ad rt t'.
 Proof.
-  intros. induction_step.
-  - admit.
-  - inversion_va. inversion_subst_clear H0. inversion_subst_clear H1.
-    destruct (Nat.eq_dec ad (length m)); subst; eauto using ForallRefs.
-    specialize (H (length m)). shelve.
-  -
-  
-  eauto using vr_con_new, vr_con_load.
-  - intros ? Hhasad. inversion_subst_clear Hhasad. eauto using ForallRefs.
-  - intros ? Hhasad. inversion_subst_clear Hhasad. admit.
+  intros * ? Hconrefs ?.
+  induction_step; inversion Hconrefs; subst; eauto using ConsistentRefs.
 Qed.
 
+Local Lemma step_alloc_vr_preservation2 : forall t t' ad v T,
+  empty |-- t is T ->
+  t --[EF_Alloc ad v]--> t' ->
+  exists rt, ConsistentRefs ad rt t'.
+Proof.
+  intros. generalize dependent T. induction_step; intros; inversion_type;
+  eauto using ConsistentRefs;
+  match goal with
+  | H : empty |-- ?t is ?T |- _ => destruct (IHstep eq_refl T H); trivial
+  end;
+  eauto using ConsistentRefs; eexists;
+  match goal with
+  | _ : ConsistentRefs _ _ ?t1 |- ConsistentRefs _ _ (_ ?t1 ?t2) => 
+    destruct (hasad_dec ad t2); eauto using nha_then_conrefs, ConsistentRefs
+  | _ : ConsistentRefs _ _ ?t2 |- ConsistentRefs _ _ (_ ?t1 ?t2) => 
+    destruct (hasad_dec ad t1); eauto using nha_then_conrefs, ConsistentRefs
+  end;
+  exfalso.
+  (* TODO *)
+Qed.
 
 Local Lemma mstep_vr_preservation : forall rt m m' t t' eff,
   valid_references rt m t ->
